PackageCalculus/Extensions/Concurrent/Lifting/Soundness.lean
@@ -16,10 +16,9 @@ theorem liftResolution_soundness
     (S' : Finset (Package N' V'))
     (hres : IsResolution (concurrentReal R_C Δ_C g) (concurrentDeps Δ_C g)
       (embedPkg g r) S')
-    (hfunc : Δ_C.FunctionalInName)
-    (hne_dep : Δ_C.NonEmpty) :
+    (hfunc : Δ_C.FunctionalInName) :
     ∃ π, IsConcurrentResolution R_C Δ_C g r (liftResolution g S') π := by
-  have hsound := concurrent_soundness R_C Δ_C g r S' hres hfunc hne_dep
+  have hsound := concurrent_soundness R_C Δ_C g r S' hres hfunc
   -- The preimageS used internally equals our liftResolution extensionally
   suffices heq : liftResolution g S' = S'.preimage (embedPkg g)
       (Set.InjOn.mono (Set.subset_univ _)
