PackageCalculus/Versions/Lifting/Completeness.lean
@@ -13,11 +13,10 @@ variable {N : Type*} [DecidableEq N]
     the original concrete `Δ`. -/
 theorem liftResolution_completeness [LinearOrder V]
     (R : Real N V) (Δ : DepRel N V) (r : Package N V) (S : Finset (Package N V))
-    (hne : Δ.NonEmpty)
     (hsub : Δ.DependeesExist R)
     (hres : IsVFResolution R (liftVFDeps R Δ) r S) :
     IsResolution R Δ r S := by
-  rw [← liftVFDeps_vfReduce R Δ hne hsub]
+  rw [← liftVFDeps_vfReduce R Δ hsub]
   exact (version_formula_correct R (liftVFDeps R Δ) r S).mpr hres
 
 end PackageCalculus
