PackageCalculus/Versions/Lifting/Soundness.lean
@@ -15,12 +15,11 @@ variable {N : Type*} [DecidableEq N]
     lifted `VFDepRel`. -/
 theorem liftResolution_soundness [LinearOrder V]
     (R : Real N V) (Δ : DepRel N V) (r : Package N V) (S : Finset (Package N V))
-    (hne : Δ.NonEmpty)
     (hsub : Δ.DependeesExist R)
     (hres : IsResolution R Δ r S) :
     IsVFResolution R (liftVFDeps R Δ) r S := by
   rw [← version_formula_correct]
-  rw [liftVFDeps_vfReduce R Δ hne hsub]
+  rw [liftVFDeps_vfReduce R Δ hsub]
   exact hres
 
 end PackageCalculus
